Update to use proper oracle

proof/refine/RISCV64/New_R.thy
@@ -12,7 +12,7 @@ axiomatization colourOracle :: "domain \<Rightarrow> obj_ref set"
 
 context begin interpretation Arch .
 
-section \<open>Domain Colour Lemmas\<close>
+section \<open>Colour Oracle Defn + Lemma\<close>
 
 definition isInDomainColour' :: "domain \<Rightarrow> machine_word \<Rightarrow> bool"
   where "isInDomainColour' d p \<equiv> p \<in> colourOracle d"
@@ -22,51 +22,64 @@ lemma colour_invariant_isInDomColour':
   "\<lbrakk>(s, s')\<in>state_relation; ptr \<in> colour_oracle (cur_domain s)\<rbrakk> \<Longrightarrow> isInDomainColour' (ksCurDomain s') ptr"
   by (simp add: isInDomainColour'_def oracle_corres curdomain_relation)
 
-lemma colour_invariant_isInDomColour:
-  "\<lbrakk>(s, s')\<in>state_relation; ptr \<in> colour_oracle (cur_domain s)\<rbrakk> \<Longrightarrow> isInDomainColour (ksCurDomain s') ptr"
-  by (simp add: isInDomainColour_def)
+section \<open>Modified Method Defns\<close>
 
-lemma getObjectInCurDomain_state_assert:
-  "getObjectInCurDomain ptr \<equiv> (do
+consts' getObjectColoured :: "machine_word \<Rightarrow> ('a :: pspace_storable) kernel"
+defs getObjectColoured_def:
+"getObjectColoured ptr \<equiv> (do
         map \<leftarrow> gets $ psMap \<circ> ksPSpace;
         (before, after) \<leftarrow> return ( lookupAround2 (fromPPtr ptr) map);
         (ptr', val) \<leftarrow> maybeToMonad before;
-        stateAssert (\<lambda>s. isInDomainColour (ksCurDomain s) ptr') [];
+        ksCurDomain \<leftarrow> gets ksCurDomain;
+        haskell_assert (isInDomainColour' ksCurDomain ptr') [];
         loadObject (fromPPtr ptr) ptr' after val
-  od)"
-  by (simp add: getObjectInCurDomain_def stateAssert_def state_assert_def bind_assoc gets_def)
+od)"
 
-lemma setObjectInCurDomain_state_assert:
-  "setObjectInCurDomain ptr val\<equiv> (do
-          ps \<leftarrow> gets ksPSpace;
-          map \<leftarrow> return ( psMap ps);
-          (before, after) \<leftarrow> return ( lookupAround2 (fromPPtr ptr) map);
-          (ptr', obj) \<leftarrow> maybeToMonad before;
-          stateAssert (\<lambda>s. isInDomainColour (ksCurDomain s) ptr') [];
-          obj' \<leftarrow> updateObject val obj (fromPPtr ptr) ptr' after;
-          map' \<leftarrow> return ( data_map_insert ptr' obj' map);
-          ps' \<leftarrow> return ( ps \<lparr> psMap := map' \<rparr>);
-          modify (\<lambda> ks. ks \<lparr> ksPSpace := ps'\<rparr>)
-  od)"
-  by (simp add: setObjectInCurDomain_def stateAssert_def state_assert_def bind_assoc gets_def)
+consts' setObjectColoured :: "machine_word \<Rightarrow> ('a :: pspace_storable) \<Rightarrow> unit kernel"
+defs setObjectColoured_def:
+"setObjectColoured ptr val\<equiv> (do
+        ps \<leftarrow> gets ksPSpace;
+        map \<leftarrow> return ( psMap ps);
+        (before, after) \<leftarrow> return ( lookupAround2 (fromPPtr ptr) map);
+        (ptr', obj) \<leftarrow> maybeToMonad before;
+        ksCurDomain \<leftarrow> gets ksCurDomain;
+        haskell_assert (isInDomainColour' ksCurDomain ptr') [];
+        obj' \<leftarrow> updateObject val obj (fromPPtr ptr) ptr' after;
+        map' \<leftarrow> return ( data_map_insert ptr' obj' map);
+        ps' \<leftarrow> return ( ps \<lparr> psMap := map' \<rparr>);
+        modify (\<lambda> ks. ks \<lparr> ksPSpace := ps'\<rparr>)
+od)"
+
+consts' getCTEColoured :: "machine_word \<Rightarrow> cte kernel"
+defs getCTEColoured_def:
+"getCTEColoured \<equiv> getObjectColoured"
+
+
+consts' threadSetInCurDomain :: "(tcb \<Rightarrow> tcb) \<Rightarrow> machine_word \<Rightarrow> unit kernel"
+defs threadSetInCurDomain_def:
+"threadSetInCurDomain f tptr \<equiv>
+    do
+       tcb <- getObjectColoured tptr;
+       setObjectColoured tptr $ f tcb
+    od"
 
 section \<open>Modified lemmas for methods\<close>
 
-lemma getObjectInCurDomain_inv [wp]:
+lemma getObjectColoured_inv [wp]:
   assumes x: "\<And>p q n ko. \<lbrace>P\<rbrace> loadObject p q n ko \<lbrace>\<lambda>(rv :: 'a :: pspace_storable). P\<rbrace>"
-  shows      "\<lbrace>P\<rbrace> getObjectInCurDomain p \<lbrace>\<lambda>(rv :: 'a :: pspace_storable). P\<rbrace>"
-  by (simp add: getObjectInCurDomain_def split_def | wp x)+
+  shows      "\<lbrace>P\<rbrace> getObjectColoured p \<lbrace>\<lambda>(rv :: 'a :: pspace_storable). P\<rbrace>"
+  by (simp add: getObjectColoured_def split_def | wp x)+
 
-lemma getObjectInCurDomain_inv_tcb [wp]:
-  "\<lbrace>P\<rbrace> getObjectInCurDomain l \<lbrace>\<lambda>(rv :: Structures_H.tcb). P\<rbrace>"
-  apply (rule getObjectInCurDomain_inv)
+lemma getObjectColoured_inv_tcb [wp]:
+  "\<lbrace>P\<rbrace> getObjectColoured l \<lbrace>\<lambda>(rv :: Structures_H.tcb). P\<rbrace>"
+  apply (rule getObjectColoured_inv)
   apply simp
   apply (rule loadObject_default_inv)
   done
 
-lemma no_fail_getObjectInCurDomain_tcb [wp]:
-  "no_fail (tcb_at' t and (\<lambda>s. isInDomainColour (ksCurDomain s) t)) (getObjectInCurDomain t :: tcb kernel)"
-  apply (simp add: getObjectInCurDomain_def split_def)
+lemma no_fail_getObjectColoured_tcb [wp]:
+  "no_fail (tcb_at' t and (\<lambda>s. isInDomainColour' (ksCurDomain s) t)) (getObjectColoured t :: tcb kernel)"
+  apply (simp add: getObjectColoured_def split_def)
   apply (rule no_fail_pre)
    apply wp
   apply (clarsimp simp add: obj_at'_def objBits_simps'
@@ -85,12 +98,12 @@ lemma no_fail_getObjectInCurDomain_tcb [wp]:
   apply (simp_all del: lookupAround2_same1)
   by (fastforce split: option.split_asm simp: objBits_simps')
 
-lemma no_fail_setObjectInCurDomain_other [wp]:
+lemma no_fail_setObjectColoured_other [wp]:
   fixes ob :: "'a :: pspace_storable"
   assumes x: "updateObject ob = updateObject_default ob"
-  shows "no_fail (obj_at' (\<lambda>k::'a. objBits k = objBits ob) ptr and (\<lambda>s. isInDomainColour (ksCurDomain s) ptr))
-                  (setObjectInCurDomain ptr ob)"
-  apply (simp add: setObjectInCurDomain_def x split_def updateObject_default_def
+  shows "no_fail (obj_at' (\<lambda>k::'a. objBits k = objBits ob) ptr and (\<lambda>s. isInDomainColour' (ksCurDomain s) ptr))
+                  (setObjectColoured ptr ob)"
+  apply (simp add: setObjectColoured_def x split_def updateObject_default_def
                    projectKO_def2 alignCheck_def alignError_def)
   apply (rule no_fail_pre)
    apply wp
@@ -107,7 +120,7 @@ lemma no_fail_setObjectInCurDomain_other [wp]:
   done
 
 lemma no_fail_setObject_tcb [wp]:
-  "no_fail (tcb_at' t and (\<lambda>s. isInDomainColour (ksCurDomain s) t)) (setObjectInCurDomain t (t'::tcb))"
+  "no_fail (tcb_at' t and (\<lambda>s. isInDomainColour' (ksCurDomain s) t)) (setObjectColoured t (t'::tcb))"
   apply (rule no_fail_pre, wp)
    apply (rule ext)+
    apply simp
@@ -130,17 +143,101 @@ thm spec_corres_split'
 thm stronger_corres_guard_imp
 find_theorems "corres"
 
+lemma no_fail_getCTE_inCurDomain [wp]:
+  "no_fail (cte_at' p and (\<lambda>s. isInDomainColour' (ksCurDomain s) p)) (getCTEColoured p)"
+  apply (simp add: getCTEColoured_def getObjectColoured_def split_def
+                   loadObject_cte alignCheck_def unless_def
+                   alignError_def is_aligned_mask[symmetric]
+             cong: kernel_object.case_cong)
+  apply (rule no_fail_pre, (wp | wpc)+)
+  apply (clarsimp simp: cte_wp_at'_def getObject_def
+                        loadObject_cte split_def in_monad
+                 dest!: in_singleton
+             split del: if_split)
+  apply (clarsimp simp: in_monad typeError_def objBits_simps
+                        magnitudeCheck_def
+                 split: kernel_object.split_asm if_split_asm option.split_asm
+             split del: if_split)
+  apply auto (* simp+ satisfies the non-domain-colour subgoals *)
+  done
+sorry
+
+lemma getCTE_inv_inCurDomain [wp]: "\<lbrace>P\<rbrace> getCTEColoured addr \<lbrace>\<lambda>rv. P\<rbrace>"
+  apply (wpsimp simp: getCTEColoured_def)
+  apply (simp add: loadObject_cte)
+  apply (case_tac ko)
+  apply safe
+  by wpsimp+
+
+lemma getObject_cte_inv_inCurDomain [wp]: "\<lbrace>P\<rbrace> (getObjectColoured addr :: cte kernel) \<lbrace>\<lambda>rv. P\<rbrace>"
+  apply (simp add: getObjectColoured_def loadObject_cte split_def)
+  apply (clarsimp simp: valid_def in_monad)
+  apply (clarsimp simp: typeError_def in_monad magnitudeCheck_def
+                 split: kernel_object.split_asm if_split_asm option.split_asm)
+  done
+
+lemma getObject_cte_det_inCurDomain: (* TODO: update cte_wp_at' to use curDomain version of getObject *)
+  "(r::cte,s') \<in> fst (getObjectColoured p s) \<Longrightarrow> fst (getObject p s) = {(r,s)} \<and> s' = s"
+  apply (clarsimp simp add: getObjectColoured_def bind_def get_def gets_def
+                            return_def loadObject_cte split_def)
+  apply (clarsimp split: kernel_object.split_asm if_split_asm option.split_asm
+                   simp: in_monad typeError_def alignError_def magnitudeCheck_def)
+       apply (simp_all add: bind_def return_def assert_opt_def split_def
+                            alignCheck_def is_aligned_mask[symmetric]
+                            unless_def when_def magnitudeCheck_def)
+  done
+sorry (* broken for same reason as no_fail - need restriction on domains being aligned *)
+
+lemma getCTE_cte_wp_at_inCurDomain:
+  "\<lbrace>\<top>\<rbrace> getCTEColoured p \<lbrace>\<lambda>rv. cte_wp_at' (\<lambda>c. c = rv) p\<rbrace>"
+  apply (clarsimp simp: valid_def cte_wp_at'_def getCTEColoured_def)
+  apply (frule state_unchanged [OF getObject_cte_inv_inCurDomain])
+  apply simp
+  apply (drule getObject_cte_det_inCurDomain, simp)
+  done
+
+lemma getCTE_sp_inCurDomain:
+  "\<lbrace>P\<rbrace> getCTEColoured p \<lbrace>\<lambda>rv. cte_wp_at' (\<lambda>c. c = rv) p and P\<rbrace>"
+  apply (rule hoare_chain)
+    apply (rule hoare_vcg_conj_lift)
+     apply (rule getCTE_cte_wp_at_inCurDomain)
+    apply (rule getCTE_inv_inCurDomain)
+   apply (rule conjI, rule TrueI, assumption)
+  apply simp
+  done
+
+lemma getObject_obj_at'_inCurDomain:
+  assumes x: "\<And>q n ko. loadObject p q n ko =
+                (loadObject_default p q n ko :: ('a :: pspace_storable) kernel)"
+  assumes P: "\<And>(v::'a::pspace_storable). (1 :: machine_word) < 2 ^ (objBits v)"
+  shows      "\<lbrace> \<top> \<rbrace> getObjectColoured p \<lbrace>\<lambda>r::'a::pspace_storable. obj_at' ((=) r) p\<rbrace>"
+  by (clarsimp simp: valid_def getObjectColoured_def in_monad
+                     loadObject_default_def obj_at'_def
+                     split_def in_magnitude_check lookupAround2_char1
+                     x P project_inject objBits_def[symmetric])
+
+lemma getObject_ko_at_inCurDomain:
+  assumes x: "\<And>q n ko. loadObject p q n ko =
+                (loadObject_default p q n ko :: ('a :: pspace_storable) kernel)"
+  assumes P: "\<And>(v::'a::pspace_storable). (1 :: machine_word) < 2 ^ (objBits v)"
+  shows      "\<lbrace> \<top> \<rbrace> getObjectColoured p \<lbrace>\<lambda>r::'a::pspace_storable. ko_at' r p\<rbrace>"
+  by (subst eq_commute, rule getObject_obj_at'_inCurDomain [OF x P])
+
+lemma getObject_ko_at_tcb_inCurDomain [wp]:
+  "\<lbrace>\<top>\<rbrace> getObjectColoured p \<lbrace>\<lambda>rv::tcb. ko_at' rv p\<rbrace>"
+  by (rule getObject_ko_at_inCurDomain | simp add: objBits_simps')+
+
 section \<open>corres lemmas\<close>
 
 lemma corres_get_tcb_inCurDomain':
-  "corres (tcb_relation \<circ> the) (tcb_at t) (tcb_at' t and (\<lambda>s. isInDomainColour (ksCurDomain s) t)) (gets (get_tcb t)) (getObjectInCurDomain t)"
+  "corres (tcb_relation \<circ> the) (tcb_at t) (tcb_at' t and (\<lambda>s. isInDomainColour' (ksCurDomain s) t)) (gets (get_tcb t)) (getObjectColoured t)"
     apply (rule corres_no_failI)
    apply wp
   apply (clarsimp simp add: gets_def get_def return_def bind_def get_tcb_def)
-  apply (frule in_inv_by_hoareD [OF getObjectInCurDomain_inv_tcb])
+  apply (frule in_inv_by_hoareD [OF getObjectColoured_inv_tcb])
   apply (clarsimp simp add: obj_at_def is_tcb obj_at'_def projectKO_def
                             projectKO_opt_tcb split_def
-                            getObjectInCurDomain_def loadObject_default_def in_monad)
+                            getObjectColoured_def loadObject_default_def in_monad)
   apply (case_tac bb)
    apply (simp_all add: fail_def return_def)
   apply (clarsimp simp add: state_relation_def pspace_relation_def)
@@ -153,14 +250,14 @@ lemma corres_get_tcb_inCurDomain':
 lemma corres_get_tcb_inCurDomain:
   "corres (tcb_relation \<circ> the)
     (tcb_at t and (\<lambda>s. t \<in> colour_oracle (cur_domain s))) (tcb_at' t)
-  (gets (get_tcb t)) (getObjectInCurDomain t)"
-  apply (rule stronger_corres_guard_imp[where Q="tcb_at t" and Q'="tcb_at' t and (\<lambda>s. isInDomainColour (ksCurDomain s) t)"])
-  by (simp add: corres_get_tcb_inCurDomain' colour_invariant_isInDomColour)+
+  (gets (get_tcb t)) (getObjectColoured t)"
+  apply (rule stronger_corres_guard_imp[where Q="tcb_at t" and Q'="tcb_at' t and (\<lambda>s. isInDomainColour' (ksCurDomain s) t)"])
+  by (simp add: corres_get_tcb_inCurDomain' colour_invariant_isInDomColour')+
 
 lemma getObject_TCB_corres_inCurDomain':
-  "corres tcb_relation (tcb_at t and pspace_aligned and pspace_distinct) (\<lambda>s. isInDomainColour (ksCurDomain s) t)
-          (gets_the (get_tcb t)) (getObjectInCurDomain t)"
-  apply (rule corres_cross_over_guard[where Q="tcb_at' t and (\<lambda>s. isInDomainColour (ksCurDomain s) t)"])
+  "corres tcb_relation (tcb_at t and pspace_aligned and pspace_distinct) (\<lambda>s. isInDomainColour' (ksCurDomain s) t)
+          (gets_the (get_tcb t)) (getObjectColoured t)"
+  apply (rule corres_cross_over_guard[where Q="tcb_at' t and (\<lambda>s. isInDomainColour' (ksCurDomain s) t)"])
    apply (fastforce simp: tcb_at_cross state_relation_def)
   apply (rule corres_guard_imp)
     apply (rule corres_gets_the)
@@ -171,17 +268,17 @@ lemma getObject_TCB_corres_inCurDomain':
 
 lemma getObject_TCB_corres_inCurDomain:
   "corres tcb_relation (tcb_at t and pspace_aligned and pspace_distinct and (\<lambda>s. t \<in> colour_oracle (cur_domain s))) \<top>
-          (gets_the (get_tcb t)) (getObjectInCurDomain t)"
-  apply (rule stronger_corres_guard_imp[where Q="tcb_at t and pspace_aligned and pspace_distinct" and Q'="\<lambda>s. isInDomainColour (ksCurDomain s) t"])
-  by (simp add: getObject_TCB_corres_inCurDomain' colour_invariant_isInDomColour)+
+          (gets_the (get_tcb t)) (getObjectColoured t)"
+  apply (rule stronger_corres_guard_imp[where Q="tcb_at t and pspace_aligned and pspace_distinct" and Q'="\<lambda>s. isInDomainColour' (ksCurDomain s) t"])
+  by (simp add: getObject_TCB_corres_inCurDomain' colour_invariant_isInDomColour')+
 
 lemma getObject_ASIDPool_corres_inCurDomain':
   "p' = p \<Longrightarrow>
    corres (\<lambda>p p'. p = inv ASIDPool p' o ucast)
-          (asid_pool_at p and pspace_aligned and pspace_distinct) (\<lambda>s. isInDomainColour (ksCurDomain s) p')
-          (get_asid_pool p) (getObjectInCurDomain p')"
+          (asid_pool_at p and pspace_aligned and pspace_distinct) (\<lambda>s. isInDomainColour' (ksCurDomain s) p')
+          (get_asid_pool p) (getObjectColoured p')"
   apply (rule corres_cross_over_asid_pool_at, fastforce)
-  apply (simp add: getObjectInCurDomain_def gets_map_def split_def)
+  apply (simp add: getObjectColoured_def gets_map_def split_def)
   apply (rule corres_no_failI)
    apply (rule no_fail_pre, wp)
    apply (clarsimp simp: typ_at'_def ko_wp_at'_def)
@@ -211,16 +308,16 @@ lemma getObject_ASIDPool_corres_inCurDomain:
   "p' = p \<Longrightarrow>
    corres (\<lambda>p p'. p = inv ASIDPool p' o ucast)
           (asid_pool_at p and pspace_aligned and pspace_distinct and (\<lambda>s. p \<in> colour_oracle (cur_domain s))) \<top>
-          (get_asid_pool p) (getObjectInCurDomain p')"
-  apply (rule stronger_corres_guard_imp[where Q="asid_pool_at p and pspace_aligned and pspace_distinct" and Q'="\<lambda>s. isInDomainColour (ksCurDomain s) p'"])
-  by (simp add: getObject_ASIDPool_corres_inCurDomain' colour_invariant_isInDomColour)+
+          (get_asid_pool p) (getObjectColoured p')"
+  apply (rule stronger_corres_guard_imp[where Q="asid_pool_at p and pspace_aligned and pspace_distinct" and Q'="\<lambda>s. isInDomainColour' (ksCurDomain s) p'"])
+  by (simp add: getObject_ASIDPool_corres_inCurDomain' colour_invariant_isInDomColour')+
 
 lemma getObject_PTE_corres_inCurDomain':
   "p = p' \<Longrightarrow>
-   corres pte_relation' (pte_at p and pspace_aligned and pspace_distinct) (\<lambda>s. isInDomainColour (ksCurDomain s) p')
-          (get_pte p) (getObjectInCurDomain p')"
+   corres pte_relation' (pte_at p and pspace_aligned and pspace_distinct) (\<lambda>s. isInDomainColour' (ksCurDomain s) p')
+          (get_pte p) (getObjectColoured p')"
   apply (rule corres_cross_over_pte_at, fastforce)
-  apply (simp add: getObjectInCurDomain_def gets_map_def split_def bind_assoc)
+  apply (simp add: getObjectColoured_def gets_map_def split_def bind_assoc)
   apply (rule corres_no_failI)
    apply (rule no_fail_pre, wp)
    apply (clarsimp simp: ko_wp_at'_def typ_at'_def lookupAround2_known1)
@@ -248,9 +345,9 @@ lemma getObject_PTE_corres_inCurDomain':
 lemma getObject_PTE_corres_inCurDomain[corres]:
   "p = p' \<Longrightarrow>
    corres pte_relation' (pte_at p and pspace_aligned and pspace_distinct and (\<lambda>s. p \<in> colour_oracle (cur_domain s))) \<top>
-          (get_pte p) (getObjectInCurDomain p')"
-  apply (rule stronger_corres_guard_imp[where Q="pte_at p and pspace_aligned and pspace_distinct" and Q'="\<lambda>s. isInDomainColour (ksCurDomain s) p'"])
-  by (simp add: getObject_PTE_corres_inCurDomain' colour_invariant_isInDomColour)+
+          (get_pte p) (getObjectColoured p')"
+  apply (rule stronger_corres_guard_imp[where Q="pte_at p and pspace_aligned and pspace_distinct" and Q'="\<lambda>s. isInDomainColour' (ksCurDomain s) p'"])
+  by (simp add: getObject_PTE_corres_inCurDomain' colour_invariant_isInDomColour')+
 
 lemma setObject_update_TCB_corres_inCurDomain'':
   assumes tcbs: "tcb_relation tcb tcb' \<Longrightarrow> tcb_relation new_tcb new_tcb'"
@@ -262,8 +359,8 @@ lemma setObject_update_TCB_corres_inCurDomain'':
   assumes r: "r () ()"
   shows
     "corres r
-       (ko_at (TCB tcb) ptr) (ko_at' tcb' ptr and (\<lambda>s. isInDomainColour (ksCurDomain s) ptr))
-       (set_object ptr (TCB new_tcb)) (setObjectInCurDomain ptr new_tcb')"
+       (ko_at (TCB tcb) ptr) (ko_at' tcb' ptr and (\<lambda>s. isInDomainColour' (ksCurDomain s) ptr))
+       (set_object ptr (TCB new_tcb)) (setObjectColoured ptr new_tcb')"
   apply (rule_tac F="tcb_relation tcb tcb'" in corres_req)
    apply (clarsimp simp: state_relation_def obj_at_def obj_at'_def)
    apply (frule(1) pspace_relation_absD)
@@ -271,7 +368,7 @@ lemma setObject_update_TCB_corres_inCurDomain'':
   apply (rule corres_no_failI)
    apply wp
    apply (clarsimp simp: obj_at'_def)
-  apply (unfold set_object_def setObjectInCurDomain_def)
+  apply (unfold set_object_def setObjectColoured_def)
   apply (clarsimp simp: in_monad split_def bind_def gets_def get_def Bex_def
                         put_def return_def modify_def get_object_def obj_at_def
                         updateObject_default_def in_magnitude_check objBits_less_word_bits)
@@ -333,8 +430,8 @@ lemma setObject_update_TCB_corres_inCurDomain':
      \<And>d p. inQ d p new_tcb' = inQ d p tcb';
      r () ()\<rbrakk> \<Longrightarrow>
    corres r
-     (\<lambda>s. get_tcb ptr s = Some tcb) ((\<lambda>s'. (tcb', s') \<in> fst (getObject ptr s')) and (\<lambda>s. isInDomainColour (ksCurDomain s) ptr))
-     (set_object ptr (TCB new_tcb)) (setObjectInCurDomain ptr new_tcb')"
+     (\<lambda>s. get_tcb ptr s = Some tcb) ((\<lambda>s'. (tcb', s') \<in> fst (getObject ptr s')) and (\<lambda>s. isInDomainColour' (ksCurDomain s) ptr))
+     (set_object ptr (TCB new_tcb)) (setObjectColoured ptr new_tcb')"
   apply (rule corres_guard_imp)
     apply (erule (4) setObject_update_TCB_corres_inCurDomain'')
    apply (clarsimp simp: getObject_def in_monad split_def obj_at'_def
@@ -350,9 +447,9 @@ lemma setObject_update_TCB_corres_inCurDomain:
      r () ()\<rbrakk> \<Longrightarrow>
    corres r
      ((\<lambda>s. get_tcb ptr s = Some tcb) and (\<lambda>s. ptr \<in> colour_oracle (cur_domain s))) ((\<lambda>s'. (tcb', s') \<in> fst (getObject ptr s')))
-     (set_object ptr (TCB new_tcb)) (setObjectInCurDomain ptr new_tcb')"
-  apply (rule stronger_corres_guard_imp[where Q="\<lambda>s. get_tcb ptr s = Some tcb" and Q'="(\<lambda>s'. (tcb', s') \<in> fst (getObject ptr s')) and (\<lambda>s. isInDomainColour (ksCurDomain s) ptr)"])
-  by (simp add: setObject_update_TCB_corres_inCurDomain' colour_invariant_isInDomColour)+
+     (set_object ptr (TCB new_tcb)) (setObjectColoured ptr new_tcb')"
+  apply (rule stronger_corres_guard_imp[where Q="\<lambda>s. get_tcb ptr s = Some tcb" and Q'="(\<lambda>s'. (tcb', s') \<in> fst (getObject ptr s')) and (\<lambda>s. isInDomainColour' (ksCurDomain s) ptr)"])
+  by (simp add: setObject_update_TCB_corres_inCurDomain' colour_invariant_isInDomColour')+
 
 lemma setObject_other_corres_inCurDomain':
   assumes x: "updateObject ob' = updateObject_default ob'"
@@ -363,15 +460,15 @@ lemma setObject_other_corres_inCurDomain':
   assumes P: "\<And>(v::'a::pspace_storable). (1 :: machine_word) < 2 ^ (objBits v)"
   shows      "other_obj_relation ob (injectKO (ob' :: 'a :: pspace_storable)) \<Longrightarrow>
   corres dc (obj_at (\<lambda>ko. a_type ko = a_type ob) ptr and obj_at (same_caps ob) ptr)
-            (obj_at' (P :: 'a \<Rightarrow> bool) ptr and (\<lambda>s. isInDomainColour (ksCurDomain s) ptr))
-            (set_object ptr ob) (setObjectInCurDomain ptr ob')"
+            (obj_at' (P :: 'a \<Rightarrow> bool) ptr and (\<lambda>s. isInDomainColour' (ksCurDomain s) ptr))
+            (set_object ptr ob) (setObjectColoured ptr ob')"
   supply image_cong_simp [cong del] projectKOs[simp del]
   apply (rule corres_no_failI)
    apply (rule no_fail_pre)
     apply wp
     apply (rule x)
    apply (clarsimp simp: b elim!: obj_at'_weakenE)
-  apply (unfold set_object_def setObjectInCurDomain_def)
+  apply (unfold set_object_def setObjectColoured_def)
   apply (clarsimp simp: in_monad split_def bind_def gets_def get_def Bex_def
                         put_def return_def modify_def get_object_def x
                         projectKOs obj_at_def
@@ -427,16 +524,16 @@ lemma setObject_other_corres_inCurDomain:
   shows      "other_obj_relation ob (injectKO (ob' :: 'a :: pspace_storable)) \<Longrightarrow>
   corres dc (obj_at (\<lambda>ko. a_type ko = a_type ob) ptr and obj_at (same_caps ob) ptr and (\<lambda>s. ptr \<in> colour_oracle (cur_domain s)))
             (obj_at' (P :: 'a \<Rightarrow> bool) ptr)
-            (set_object ptr ob) (setObjectInCurDomain ptr ob')"
-  apply (rule stronger_corres_guard_imp[where Q="obj_at (\<lambda>ko. a_type ko = a_type ob) ptr and obj_at (same_caps ob) ptr" and Q'="obj_at' (P :: 'a \<Rightarrow> bool) ptr  and (\<lambda>s. isInDomainColour (ksCurDomain s) ptr)"])
-  by (simp add: setObject_other_corres_inCurDomain' colour_invariant_isInDomColour x z t b P)+
+            (set_object ptr ob) (setObjectColoured ptr ob')"
+  apply (rule stronger_corres_guard_imp[where Q="obj_at (\<lambda>ko. a_type ko = a_type ob) ptr and obj_at (same_caps ob) ptr" and Q'="obj_at' (P :: 'a \<Rightarrow> bool) ptr  and (\<lambda>s. isInDomainColour' (ksCurDomain s) ptr)"])
+  by (simp add: setObject_other_corres_inCurDomain' colour_invariant_isInDomColour' x z t b P)+
 
 lemma setObject_PT_corres_inCurDomain':
   "pte_relation' pte pte' \<Longrightarrow>
    corres dc ((\<lambda>s. pts_of s (table_base p) = Some pt) and K (is_aligned p pte_bits) and
-              pspace_aligned and pspace_distinct) (\<lambda>s. isInDomainColour (ksCurDomain s) p)
+              pspace_aligned and pspace_distinct) (\<lambda>s. isInDomainColour' (ksCurDomain s) p)
           (set_pt (table_base p) (pt(table_index p := pte)))
-          (setObjectInCurDomain p pte')"
+          (setObjectColoured p pte')"
   supply opt_mapE[elim!]
   apply (rule corres_cross_over_pte_at[where p=p])
    apply (simp add: pte_at_eq ptes_of_def in_omonad)
@@ -449,7 +546,7 @@ lemma setObject_PT_corres_inCurDomain':
    apply (rename_tac arch_kernel_object)
    apply (case_tac arch_kernel_object; simp)
    apply (simp add: objBits_simps word_bits_def)
-  apply (clarsimp simp: setObjectInCurDomain_def in_monad split_def updateObject_default_def)
+  apply (clarsimp simp: setObjectColoured_def in_monad split_def updateObject_default_def)
   apply (simp add: in_magnitude_check objBits_simps a_type_simps)
   apply (clarsimp simp: obj_at_def exec_gets a_type_simps opt_map_def exec_get put_def)
   apply (clarsimp simp: state_relation_def mask_pt_bits_inner_beauty)
@@ -509,14 +606,14 @@ lemma setObject_PT_corres_inCurDomain:
    corres dc ((\<lambda>s. pts_of s (table_base p) = Some pt) and K (is_aligned p pte_bits) and
               pspace_aligned and pspace_distinct and (\<lambda>s. p \<in> colour_oracle (cur_domain s))) \<top>
           (set_pt (table_base p) (pt(table_index p := pte)))
-          (setObjectInCurDomain p pte')"
-  apply (rule stronger_corres_guard_imp[where Q="(\<lambda>s. pts_of s (table_base p) = Some pt) and K (is_aligned p pte_bits) and  pspace_aligned and pspace_distinct" and Q'="\<lambda>s. isInDomainColour (ksCurDomain s) p"])
-  by (simp only: setObject_PT_corres_inCurDomain'|simp add: colour_invariant_isInDomColour)+
+          (setObjectColoured p pte')"
+  apply (rule stronger_corres_guard_imp[where Q="(\<lambda>s. pts_of s (table_base p) = Some pt) and K (is_aligned p pte_bits) and  pspace_aligned and pspace_distinct" and Q'="\<lambda>s. isInDomainColour' (ksCurDomain s) p"])
+  by (simp only: setObject_PT_corres_inCurDomain'|simp add: colour_invariant_isInDomColour')+
 
 lemma setObject_ASIDPool_corres_inCurDomain':
   "\<lbrakk> a = inv ASIDPool a' o ucast; p' = p \<rbrakk> \<Longrightarrow>
-  corres dc (asid_pool_at p and pspace_aligned and pspace_distinct) (\<lambda>s. isInDomainColour (ksCurDomain s) p')
-            (set_asid_pool p a) (setObjectInCurDomain p' a')"
+  corres dc (asid_pool_at p and pspace_aligned and pspace_distinct) (\<lambda>s. isInDomainColour' (ksCurDomain s) p')
+            (set_asid_pool p a) (setObjectColoured p' a')"
   apply (simp add: set_asid_pool_def)
   apply (rule corres_underlying_symb_exec_l[where P=P and Q="\<lambda>_. P" for P])
     apply (rule corres_no_failI; clarsimp)
@@ -550,78 +647,15 @@ lemma setObject_ASIDPool_corres_inCurDomain':
 lemma setObject_ASIDPool_corres_inCurDomain[corres]:
   "\<lbrakk> a = inv ASIDPool a' o ucast; p' = p \<rbrakk> \<Longrightarrow>
   corres dc (asid_pool_at p and pspace_aligned and pspace_distinct and (\<lambda>s. p \<in> colour_oracle (cur_domain s))) \<top>
-            (set_asid_pool p a) (setObjectInCurDomain p' a')"
-  apply (rule stronger_corres_guard_imp[where Q="asid_pool_at p and pspace_aligned and pspace_distinct" and Q'="\<lambda>s. isInDomainColour (ksCurDomain s) p"])
-  by (simp add: colour_invariant_isInDomColour setObject_ASIDPool_corres_inCurDomain')+
-
-lemma no_fail_getCTE_inCurDomain [wp]:
-  "no_fail (cte_at' p and (\<lambda>s. isInDomainColour (ksCurDomain s) p)) (getCTEInCurDomain p)"
-  apply (simp add: getCTEInCurDomain_def getObjectInCurDomain_def split_def
-                   loadObject_cte alignCheck_def unless_def
-                   alignError_def is_aligned_mask[symmetric]
-             cong: kernel_object.case_cong)
-  apply (rule no_fail_pre, (wp | wpc)+)
-  apply (clarsimp simp: cte_wp_at'_def getObject_def
-                        loadObject_cte split_def in_monad
-                 dest!: in_singleton
-             split del: if_split)
-  apply (clarsimp simp: in_monad typeError_def objBits_simps
-                        magnitudeCheck_def
-                 split: kernel_object.split_asm if_split_asm option.split_asm
-             split del: if_split)
-  apply auto (* simp+ satisfies the non-domain-colour subgoals *)
-  done
-sorry
-
-lemma getCTE_inv_inCurDomain [wp]: "\<lbrace>P\<rbrace> getCTEInCurDomain addr \<lbrace>\<lambda>rv. P\<rbrace>"
-  apply (wpsimp simp: getCTEInCurDomain_def)
-  apply (simp add: loadObject_cte)
-  apply (case_tac ko)
-  apply safe
-  by wpsimp+
-
-lemma getObject_cte_inv_inCurDomain [wp]: "\<lbrace>P\<rbrace> (getObjectInCurDomain addr :: cte kernel) \<lbrace>\<lambda>rv. P\<rbrace>"
-  apply (simp add: getObjectInCurDomain_def loadObject_cte split_def)
-  apply (clarsimp simp: valid_def in_monad)
-  apply (clarsimp simp: typeError_def in_monad magnitudeCheck_def
-                 split: kernel_object.split_asm if_split_asm option.split_asm)
-  done
-
-lemma getObject_cte_det_inCurDomain: (* TODO: update cte_wp_at' to use curDomain version of getObject *)
-  "(r::cte,s') \<in> fst (getObjectInCurDomain p s) \<Longrightarrow> fst (getObject p s) = {(r,s)} \<and> s' = s"
-  apply (clarsimp simp add: getObjectInCurDomain_def bind_def get_def gets_def
-                            return_def loadObject_cte split_def)
-  apply (clarsimp split: kernel_object.split_asm if_split_asm option.split_asm
-                   simp: in_monad typeError_def alignError_def magnitudeCheck_def)
-       apply (simp_all add: bind_def return_def assert_opt_def split_def
-                            alignCheck_def is_aligned_mask[symmetric]
-                            unless_def when_def magnitudeCheck_def)
-  done
-sorry (* broken for same reason as no_fail - need restriction on domains being aligned *)
-
-lemma getCTE_cte_wp_at_inCurDomain:
-  "\<lbrace>\<top>\<rbrace> getCTEInCurDomain p \<lbrace>\<lambda>rv. cte_wp_at' (\<lambda>c. c = rv) p\<rbrace>"
-  apply (clarsimp simp: valid_def cte_wp_at'_def getCTEInCurDomain_def)
-  apply (frule state_unchanged [OF getObject_cte_inv_inCurDomain])
-  apply simp
-  apply (drule getObject_cte_det_inCurDomain, simp)
-  done
-
-lemma getCTE_sp_inCurDomain:
-  "\<lbrace>P\<rbrace> getCTEInCurDomain p \<lbrace>\<lambda>rv. cte_wp_at' (\<lambda>c. c = rv) p and P\<rbrace>"
-  apply (rule hoare_chain)
-    apply (rule hoare_vcg_conj_lift)
-     apply (rule getCTE_cte_wp_at_inCurDomain)
-    apply (rule getCTE_inv_inCurDomain)
-   apply (rule conjI, rule TrueI, assumption)
-  apply simp
-  done
+            (set_asid_pool p a) (setObjectColoured p' a')"
+  apply (rule stronger_corres_guard_imp[where Q="asid_pool_at p and pspace_aligned and pspace_distinct" and Q'="\<lambda>s. isInDomainColour' (ksCurDomain s) p"])
+  by (simp add: colour_invariant_isInDomColour' setObject_ASIDPool_corres_inCurDomain')+
 
 lemma get_cap_inCurDomain_corres_P':
   "corres (\<lambda>x y. cap_relation x (cteCap y) \<and> P x)
           (cte_wp_at P cslot_ptr)
-          (pspace_aligned' and pspace_distinct' and (\<lambda>s. isInDomainColour (ksCurDomain s) (cte_map cslot_ptr)))
-          (get_cap cslot_ptr) (getCTEInCurDomain (cte_map cslot_ptr))"
+          (pspace_aligned' and pspace_distinct' and (\<lambda>s. isInDomainColour' (ksCurDomain s) (cte_map cslot_ptr)))
+          (get_cap cslot_ptr) (getCTEColoured (cte_map cslot_ptr))"
 thm get_cap_corres_P
   apply (rule corres_stronger_no_failI)
    apply (rule no_fail_pre, wp)
@@ -646,9 +680,9 @@ lemma get_cap_inCurDomain_corres_P:
   "corres (\<lambda>x y. cap_relation x (cteCap y) \<and> P x)
           (cte_wp_at P cslot_ptr and (\<lambda>s. cte_map cslot_ptr \<in> colour_oracle (cur_domain s)))
           (pspace_aligned' and pspace_distinct')
-          (get_cap cslot_ptr) (getCTEInCurDomain (cte_map cslot_ptr))"
-  apply (rule stronger_corres_guard_imp[where Q="cte_wp_at P cslot_ptr" and Q'="pspace_aligned' and pspace_distinct' and (\<lambda>s. isInDomainColour (ksCurDomain s) (cte_map cslot_ptr))"])
-  by (simp add: colour_invariant_isInDomColour get_cap_inCurDomain_corres_P')+
+          (get_cap cslot_ptr) (getCTEColoured (cte_map cslot_ptr))"
+  apply (rule stronger_corres_guard_imp[where Q="cte_wp_at P cslot_ptr" and Q'="pspace_aligned' and pspace_distinct' and (\<lambda>s. isInDomainColour' (ksCurDomain s) (cte_map cslot_ptr))"])
+  by (simp add: colour_invariant_isInDomColour' get_cap_inCurDomain_corres_P')+
 
 lemmas get_cap_inCurDomain_corres = get_cap_inCurDomain_corres_P[where P="\<top>", simplified]
 
@@ -662,37 +696,6 @@ find_theorems getObjectInCurDomain name: def
 find_theorems threadSet name: def
 find_theorems threadSet corres
 
-consts'
-threadSetInCurDomain :: "(tcb \<Rightarrow> tcb) \<Rightarrow> machine_word \<Rightarrow> unit kernel"
-
-defs threadSetInCurDomain_def:
-" threadSetInCurDomain f tptr \<equiv>
-    do
-       tcb <- getObjectInCurDomain tptr;
-       setObjectInCurDomain tptr $ f tcb
-    od"
-
-lemma getObject_obj_at'_inCurDomain:
-  assumes x: "\<And>q n ko. loadObject p q n ko =
-                (loadObject_default p q n ko :: ('a :: pspace_storable) kernel)"
-  assumes P: "\<And>(v::'a::pspace_storable). (1 :: machine_word) < 2 ^ (objBits v)"
-  shows      "\<lbrace> \<top> \<rbrace> getObjectInCurDomain p \<lbrace>\<lambda>r::'a::pspace_storable. obj_at' ((=) r) p\<rbrace>"
-  by (clarsimp simp: valid_def getObjectInCurDomain_def in_monad
-                     loadObject_default_def obj_at'_def
-                     split_def in_magnitude_check lookupAround2_char1
-                     x P project_inject objBits_def[symmetric])
-
-lemma getObject_ko_at_inCurDomain:
-  assumes x: "\<And>q n ko. loadObject p q n ko =
-                (loadObject_default p q n ko :: ('a :: pspace_storable) kernel)"
-  assumes P: "\<And>(v::'a::pspace_storable). (1 :: machine_word) < 2 ^ (objBits v)"
-  shows      "\<lbrace> \<top> \<rbrace> getObjectInCurDomain p \<lbrace>\<lambda>r::'a::pspace_storable. ko_at' r p\<rbrace>"
-  by (subst eq_commute, rule getObject_obj_at'_inCurDomain [OF x P])
-
-lemma getObject_ko_at_tcb_inCurDomain [wp]:
-  "\<lbrace>\<top>\<rbrace> getObjectInCurDomain p \<lbrace>\<lambda>rv::tcb. ko_at' rv p\<rbrace>"
-  by (rule getObject_ko_at_inCurDomain | simp add: objBits_simps')+
-
 lemma threadsetInCurDomain_corresT':
   assumes x: "\<And>tcb tcb'. tcb_relation tcb tcb' \<Longrightarrow>
                          tcb_relation (f tcb) (f' tcb')"
@@ -703,7 +706,7 @@ lemma threadsetInCurDomain_corresT':
                           "\<And>tcb. tcbSchedNext (f' tcb) = tcbSchedNext tcb"
   assumes flag: "\<And>d p tcb'. inQ d p (f' tcb') = inQ d p tcb'"
   shows      "corres dc (tcb_at t and pspace_aligned and pspace_distinct)
-                        (\<lambda>s. isInDomainColour (ksCurDomain s) t)
+                        (\<lambda>s. isInDomainColour' (ksCurDomain s) t)
                         (thread_set f t) (threadSetInCurDomain f' t)"
   apply (simp add: thread_set_def threadSetInCurDomain_def)
   apply (rule corres_guard_imp)
@@ -736,8 +739,8 @@ lemma threadsetInCurDomain_corresT:
   shows      "corres dc (tcb_at t and pspace_aligned and pspace_distinct and (\<lambda>s. t \<in> colour_oracle (cur_domain s)))
                         \<top>
                         (thread_set f t) (threadSetInCurDomain f' t)"
-  apply (rule stronger_corres_guard_imp[where Q="tcb_at t and pspace_aligned and pspace_distinct" and Q'="(\<lambda>s. isInDomainColour (ksCurDomain s) t)"])
-  by (simp add: colour_invariant_isInDomColour threadsetInCurDomain_corresT' x y z sched_pointers flag)+
+  apply (rule stronger_corres_guard_imp[where Q="tcb_at t and pspace_aligned and pspace_distinct" and Q'="(\<lambda>s. isInDomainColour' (ksCurDomain s) t)"])
+  by (simp add: colour_invariant_isInDomColour' threadsetInCurDomain_corresT' x y z sched_pointers flag)+
 
 lemmas threadsetInCurDomain_corres =
     threadsetInCurDomain_corresT [OF _ _ all_tcbI, OF _ ball_tcb_cap_casesI ball_tcb_cte_casesI]
